

# Analytic Combinatorics of Unlabeled Objects

## Set of exercises IV: responses

1. For each of the following functions  $f(z)$ , find the radius of convergence and an equivalent (asymptotic) for the coefficients of the power-series expansion  $f(z) = \sum a_n z^n$  at  $z = 0$ .

(a)  $f(z) = \frac{1}{(1-2z)^2} \log\left(\frac{1}{1-z}\right)$ .

(b)  $f(z) = \frac{e^{2z}-1}{(1-z)(1-2z)^3}$ .

(c)  $f(z) = \frac{1}{2-e^z}$ .

**Response.**

- (a) The singularity closest to the origin is  $z = 1/2$ , as  $\log\left(\frac{1}{1-z}\right)$  is analytic on  $|z| < 1$ . Thus the radius of convergence is  $\rho = 1/2$ . For the asymptotics, expanding  $\log\left(\frac{1}{1-z}\right)$  around  $z = 1/2$ , we obtain  $f(z) = \frac{1}{(1-2z)^2} \log\left(\frac{1}{1-1/2}\right) + \frac{1}{(1-2z)^2} \left(\frac{1}{1-1/2}\right) (z - 1/2) + \text{analytic}$ .

That is

$$g(z) = f(z) - \left( \frac{1}{(1-2z)^2} \log 2 - \frac{1}{1-2z} \right)$$

is analytic at  $z = 1/2$ , and hence analytic on  $|z| < 1$ . It follows that, for any fixed  $\epsilon > 0$ , we have  $[z^n]g(z) = O((1+\epsilon)^n)$ . Thus

$$[z^n]f(z) = [z^n] \frac{1}{(1-2z)^2} \log 2 + [z^n] \frac{1}{1-2z} + O((1+\epsilon)^n) = (\log 2) \cdot (n+1) \cdot 2^n - 2^n + O((1+\epsilon)^n).$$

We deduce  $[z^n]f(z) \sim (\log 2)n2^n$ .

- (b) The singularity closest to the origin is  $z = 1/2$ . Thus the radius of convergence is  $\rho = 1/2$ . In this case, expanding  $\frac{e^{2z}-1}{1-z}$  around  $z = 1/2$  we obtain

$$f(z) = \frac{2(e-1)}{(1-2z)^3} + \frac{c_1}{(1-2z)^2} + \frac{c_2}{(1-2z)^1} + \text{analytic at } z = 1/2.$$

The latter analytic function, being analytic up to  $z = 1$ , it will not contribute to the dominant asymptotics. Since  $[z^n](1-z/\rho)^{-m} \sim \frac{n^{m-1}}{(m-1)!} \rho^{-n}$  for any positive integer  $m \geq 1$ ,

$$[z^n]f(z) \sim 2(e-1) \frac{n^2}{2} 2^n = (e-1)n^2 2^n.$$

- (c) The singularities satisfy  $e^z = 2$ , i.e., these are  $z = \log 2 + 2\pi i k$  with  $k \in \mathbb{Z}$ . The closest to the origin is  $\log 2$ . Thus the radius of convergence is  $\rho = \log 2$ .

Expand the power series of the denominator around  $z = \log 2$ ,

$$\frac{1}{2-e^z} = \frac{1}{(2-e^z)'_{z=\log 2} (z - \log 2) + \sum_{k \geq 2} c_k (z - \log 2)^k} = \frac{1/2}{\log 2 - z} \times \frac{1}{1 + \sum_{k \geq 1} \hat{c}_k (z - \log 2)^k}.$$

The multiplicative inverse  $(1 + \sum_{k \geq 1} \hat{c}_k (z - \log 2)^k)^{-1}$  is well-defined, since the denominator is not 0 at  $z = \log 2$ , and  $(1 + \sum_{k \geq 1} \hat{c}_k (z - \log 2)^k)^{-1} = 1 + \sum_{k \geq 1} d_k (z - \log 2)^k$  for

certain coefficients. Remark, moreover, that this expansion is entire (radius of convergence  $\infty$ ) as this is the case for  $2 - e^z$ .

Expanding

$$f(z) = \frac{1/2}{\log 2 - z} + \text{analytic at } z = \log 2.$$

Since there are no more singularities on  $|z| = \log 2$  and the function is meromorphic we deduce that

$$[z^n]f(z) \sim [z^n] \frac{1/2}{\log 2 - z} = [z^n] \frac{1/(2 \log 2)}{1 - z/\log 2} = \frac{1}{2} (\log 2)^{-(n+1)}.$$

2. In this exercise we prove a key inequality in Coding and Information Theory by using the radius of convergence.

Let  $\mathcal{A} = \{a_1, \dots, a_k\}$  and  $\mathcal{B} = \{0, 1\}$ . A **binary code**  $c: \mathcal{A}^* \rightarrow \mathcal{B}^*$  is a morphism, i.e.,  $c(xy) = c(x)c(y)$ . The code  $c$  is *uniquely decodable* iff it is injective.

(a) Let<sup>1</sup>  $A(z) = \sum_{a \in \mathcal{A}} z^{|c(a)|}$ . Show  $C(z) = \sum_{v \in c(\mathcal{A}^*)} z^{|v|} = \frac{1}{1-A(z)}$ .

(b) [**Kraft-McMillan inequality**] Prove that if  $c$  is uniquely decodable, then

$$\sum_{a \in \mathcal{A}} 2^{-|c(a)|} \leq 1.$$

**Hint.** Reason by contradiction. Note that power-series are continuous within their radius of convergence.

(c) [**Shannon bound**] (Optional) Consider a distribution  $\mathbf{p} = (p_1, \dots, p_k)$  over  $(a_1, \dots, a_k)$ . Prove that, for a random symbol  $X$ ,

$$H(\mathbf{p}) = \sum_{j=1}^k p_j \log_2(1/p_j) \leq \sum_{j=1}^k p_j |c(a_j)| = \mathbb{E}[c(X)].$$

**Hint.** Prove that  $\log x \leq x - 1$  for all  $x \in \mathbb{R}_{>0}$ . Use the Kraft-McMillan inequality.

**Response.**

(a) Since  $c$  is a morphism, any element  $v \in c(\mathcal{A}^*)$  can be seen as a *sequence* of elements from  $c(\mathcal{A})$ , whose OGF is  $A(z)$ , thus  $C(z) = \frac{1}{1-A(z)}$ .

(b) Suppose otherwise. Then  $A(1/2) = \sum_{a \in \mathcal{A}} 2^{-|c(a)|} > 1$ .

– By continuity of  $A(z)$  within its radius of convergence, which is infinite since  $A(z)$  is actually a polynomial because  $\mathcal{A}$  is finite, it follows that there must be  $c \in (0, 1/2)$  such that  $A(c) = 1$ . We suppose that  $c$  is the smallest such  $c > 0$ . Then  $A(t) < 1$  for  $0 \leq t < c$  and  $C(z)$  converges there. Observe that increases  $C(t) \rightarrow \infty$  as  $t \rightarrow c^-$ .

– Being  $c$  uniquely decodable, it follows that there must be at most  $2^n$  words of length  $n$  in  $c(\mathcal{A}^*)$  for each  $n \geq 0$ . Hence, for  $t \in (0, 1/2)$ , we deduce  $C(t) \leq \sum_{n=0}^{\infty} 2^n t^n = \frac{1}{1-2t}$ . This means that  $C(t) \leq \frac{1}{1-2c} < \infty$  for  $0 \leq t < c$ , a contradiction.

<sup>1</sup>Here  $|w|$  is the length of the word, i.e., the number of symbols.

- (c) We first prove the inequality  $\log x \leq x - 1$  for all  $x > 0$ . Considering  $f(x) = x - 1 - \log x$ , we have  $f'(x) = 1 - \frac{1}{x}$ . Looking at the sign of  $f'(x)$ , we deduce that  $f(x)$  decreases on  $(0, 1]$  and increases in  $[1, \infty)$ . Hence the minimum of  $f(x)$  is found at  $x = 1$ ,  $f(x) \geq f(1) = 0$  and the auxiliary inequality is proved.

The inequality we want to prove,  $H(\mathbf{p}) \leq \mathbb{E}[c(X)]$ , is equivalent to

$$\sum_j p_j \log_2(2^{-|c(a_j)|}/p_j) \leq 0.$$

By using the inequality  $\log(x) \leq x - 1$  we deduce  $\log_2(2^{-|c(a_j)|}/p_j) \leq \frac{1}{\log 2} (2^{-|c(a_j)|}/p_j - 1)$ , thus

$$\sum_j p_j \log_2(2^{-|c(a_j)|}/p_j) \leq \frac{1}{\log 2} \sum_j p_j (2^{-|c(a_j)|}/p_j - 1) = \frac{1}{\log 2} \left( \sum_j 2^{-|c(a_j)|} - \sum_j p_j \right) = 0,$$

where the last equality follows from the Kraft-inequality  $\sum_j 2^{-|c(a_j)|} \leq 1$  and the equality  $\sum_j p_j = 1$ . Thus the result is proved.

3. (a) Prove the following classical lemma:

**Daffodil Lemma.** Let  $f(z)$  be analytic on  $|z| < \rho$ , with non-negative coefficients at  $z = 0$ . If the expansion does not reduce to a single monomial and, for some  $w \neq 0$ ,  $|w| < \rho$ , we have  $f(|w|) = |f(w)|$ , then

- (a.1) we must have  $w = Re^{i\theta}$  with  $\theta/(2\pi) = \frac{r}{p}$  a rational,  $\gcd(r, p) = 1$ ,  $p > 0$ ,  
(a.2) the non-zero coefficients  $a_n = [z^n]f(z)$  occur at positions  $n$  all belonging to  $a + p\mathbb{Z}_{\geq 0}$  for some fixed  $a$ .

- (b) [The statement has been corrected] Consider the class  $\mathcal{C}$  of binary words **without**  $K$  consecutive ones, with  $K \in \mathbb{Z}_{\geq 2}$  fixed.

(b.1) Prove that  $C(z) = \frac{1+z+\dots+z^{K-1}}{1-z \times (1+z+\dots+z^{K-1})} = \frac{1-z^K}{1-2z+z^{K+1}}$ .

- (b.2) Give a polynomial equation characterizing the radius of convergence  $z = \rho_C$ . Prove that  $\rho_C$  is a simple pole of  $C(z)$ .

- (b.3) Prove that there are no other singularities on  $|z| = \rho_C$ .

- (b.4) Conclude that  $[z^n]C(z) \sim c \cdot \rho_C^{-n}$  and give an expression for  $c$  in terms of  $\rho_C$  and  $K$ .

**Note.** The Fibonacci numbers correspond to the case  $K = 2$ , then  $[z^n]C(z) = f_{n+1}$  and  $\rho_C = 1/\phi$ ,  $\phi = (1 + \sqrt{5})/2$ .

## Responses.

- (a.1) Notice that  $|f(w)| \leq f(|w|)$  holds always, due to the triangle inequality. For there to be equality, all terms of the sum in  $f(w)$  must “point” in the same direction seen as vectors in the complex plane.

Write  $f(z) = \sum a_n z^n$ . By hypothesis the coefficients  $a_n \geq 0$ , and there are at least two  $a_{n_1} > 0$  and  $a_{n_2} > 0$  with  $n_1 < n_2$ . By the previous argument we must have that  $\arg(a_{n_1} w^{n_1}) = \arg(a_{n_2} w^{n_2})$ , the angle is the same. Since the coefficients are positive, this is equivalent to  $\arg(w^{n_1}) = \arg(w^{n_2})$ . Thus, if  $w = Re^{i\theta}$ , then  $\theta n_1 \equiv \theta n_2 \pmod{2\pi}$ . Thus  $\theta(n_2 - n_1) = 2\pi m$  for some  $m \in \mathbb{Z}$  and we deduce  $\theta = 2\pi \frac{m}{n_2 - n_1}$ .

- (a.2) Here  $p > 0$  is the denominator of the reduced fraction  $\theta/(2\pi) = r/p$ . Let  $k = a$  be the smallest index<sup>2</sup> such that  $a_k > 0$ . Any index  $n$  with  $a_n > 0$  must satisfy, due to part (a) that  $\theta(n - a) \in 2\pi\mathbb{Z}$ . Using the equation for  $\theta$ , we have  $\frac{r}{p}(n - a) \in \mathbb{Z}$ , but then  $p$  must divide  $n - a$ , because  $\gcd(r, p) = 1$ . Thus  $n \in a + p\mathbb{Z}_{\geq 0}$ .
- (b.1) The class can be specified as  $\mathcal{C} = \text{Seq}(\text{Seq}_{<K}(1) \cdot 0) \cdot \text{Seq}_{<K}(1)$ , where the subscript of the sequences denote a restriction to the involved lengths. This is explained as follows: whenever there is a 0, it must be preceded by less than  $K$  1s, and there might be a tail of at most  $K - 1$  1s.

Thus it follows that the ordinary generating function is

$$C(z) = \frac{1 + z + \dots + z^{K-1}}{1 - z \times (1 + z + \dots + z^{K-1})}.$$

Using  $1 + z + \dots + z^{K-1} = \frac{1-z^K}{1-z}$  we find an alternative expression

$$C(z) = \frac{1 - z^K}{1 - 2z + z^{K+1}}.$$

Note that in this latter expression  $z = 1$  is a common root of the denominator and the numerator, and it cancels out as it is a simple root of both.

- (b.2) Looking back at the equation for  $C(z)$  before simplifying  $q_K(z) := 1 + z + \dots + z^{K-1}$ , as long as  $|zq_K(z)| < 1$  the function  $C(z)$  is analytic. By Pringsheim's Theorem, the radius of convergence of a power series with positive coefficients is itself a dominant singularity. Thus it is enough to look at the positive axes to determine  $\rho_C$ .

The singularity comes when  $\rho_C \times q_K(\rho_C) = 1$ . We note that  $\rho_C < 1$  as  $1 \times q_K(1) = K > 1$ . Since  $\rho_C \neq 1$ , from the second expression for  $C(z)$  we conclude that

$$1 - 2\rho_C + \rho_C^{K+1} = 0.$$

The polynomial  $p(x) = 1 - 2x + x^{K+1}$  has a derivative  $p'(x) = -2 + (K+1)x^K$ . If  $\rho_C$  were a double root, then  $p'(\rho_C) = 0$  and so  $\rho_C^K = \frac{2}{K+1}$ . Since  $0 = 1 - 2\rho_C + \rho_C^{K+1}$ , we deduce  $0 = 1 - 2\rho_C + \rho_C \frac{2}{K+1} = 1 - 2\rho_C(1 - 1/(K+1))$ , i.e.,  $\rho_C = (K+1)/(2K)$ .

But  $2/(K+1) = \rho_C^K$  yields  $(K+1)^{K+1} = 2^{K+1}K^K$ . Since  $\gcd(K, K+1) = 1$  and  $(K+1)^{K+1}$  divides  $2^{K+1}K^K$ ,  $(K+1)^{K+1}$  must divide  $2^{K+1}$ . However  $K+1 \geq 3$  and so  $(K+1)^{K+1} > 2^{K+1}$ , an absurd. Thus  $\rho_C$  is a simple root and the pole is simple.

- (b.3) We apply the Daffodil Lemma. Suppose  $w = \rho_C e^{i\theta}$  were a dominant singularity. Then again we must have  $w \times (1 + w + \dots + w^{K-1}) = 1$ . Let  $f(z) = z \times (1 + z + \dots + z^{K-1})$ . We have  $|f(w)| = 1 = f(\rho_C) = f(|w|)$ . Thus we are ready to apply the Lemma:  $\theta = 2\pi \cdot r/p$  for some reduced fraction with  $\gcd(r, p) = 1$  and  $p > 0$ . But (a.2) implies that, then, all non-zero coefficients of  $f(z)$  belong to  $a + p\mathbb{Z}_{\geq 0}$  for some  $a$ . Looking at  $f(z)$ , this is only possible for  $p = 1$ , and it follows that  $\theta \in 2\pi\mathbb{Z}$  and  $w = \rho_C$ . Thus there are no other dominant singularities.

---

<sup>2</sup>Sorry for the choice of the letter  $a$ ...

- 
- (b.4) The generating function  $C(z)$  is rational and  $\rho_C > 0$  is the only dominant singularity. We proved that the pole at  $z = \rho_C$  is simple, and then  $C(z) \sim \frac{c}{1-z/\rho_C}$  for some  $c \neq 0$ , as  $z \rightarrow \rho_C$ . By the principle of asymptotics of rational functions (see Section 3.2 of the notes), or the Transfer Theorem (a bit overkill, but true),  $[z^n]C(z) \sim c \cdot \rho_C^{-n}$ .

The constant  $c$  must equal

$$\lim_{z \rightarrow \rho_C} (1 - z/\rho_C)C(z) = -\frac{1}{\rho_C} \lim_{z \rightarrow \rho_C} (z - \rho_C) \frac{1 - z^K}{p(z)} = -\frac{1 - \rho_C^K}{\rho_C} \frac{1}{p'(\rho_C)} = \frac{1 - \rho_C^K}{\rho_C} \frac{1}{2 - (K + 1)\rho_C^K}.$$

**Extra.** Since  $c > 0$  by combinatorial considerations, and  $\rho_C^K < 1$ , we deduce that  $2 > (K + 1)\rho_C^K$ , i.e.,  $\sqrt[K]{2/(K + 1)} > \rho_C$ .